feat(library/bitvec): add a proof that to_nat and of_nat cancel each other

library/data/bitvec.lean
@@ -136,19 +136,48 @@ end comparison
 section conversion
   variable {α : Type}
 
+  @[reducible]
+  protected def list_of_nat : ℕ → ℕ → list bool
+  | 0        x := list.nil
+  | (succ n) x := list_of_nat n (x / 2) ++ [to_bool (x % 2 = 1)]
+
   protected def of_nat : Π (n : ℕ), nat → bitvec n
   | 0        x := nil
   | (succ n) x := of_nat n (x / 2) ++ₜ [to_bool (x % 2 = 1)]
+
+  @[simp]
+  protected lemma of_nat_to_list (m n : ℕ)
+  : (bitvec.of_nat m n)^.to_list = bitvec.list_of_nat m n :=
+  begin
+    revert n,
+    induction m with m,
+    { intro, refl },
+    { intro n, unfold list_of_nat of_nat, simp [ih_1] }
+  end
 
   protected def of_int : Π (n : ℕ), int → bitvec (succ n)
   | n (int.of_nat m)          := ff :: bitvec.of_nat n m
   | n (int.neg_succ_of_nat m) := tt :: not (bitvec.of_nat n m)
 
+  def add_lsb (r : ℕ) (b : bool) : ℕ := r + r + cond b 1 0
+
+  @[simp]
+  lemma add_lsb_zero (b : bool) : add_lsb 0 b = cond b 1 0 :=
+  begin unfold add_lsb, simp end
+
   def bits_to_nat (v : list bool) : nat :=
-  list.foldl (λ r b, r + r + cond b 1 0) 0 v
+  list.foldl add_lsb 0 v
 
   protected def to_nat {n : nat} (v : bitvec n) : nat :=
   bits_to_nat (to_list v)
+
+  @[simp]
+  lemma to_nat_eq_bits_to_nat {n : ℕ} (x : bitvec n)
+  : bitvec.to_nat x = bits_to_nat x^.to_list :=
+  begin
+    cases x with x Px,
+    refl,
+  end
 
   protected def to_int : Π {n : nat}, bitvec n → int
   | 0        _ := 0
@@ -165,6 +194,69 @@ private def to_string {n : nat} : bitvec n → string
 
 instance (n : nat) : has_to_string (bitvec n) :=
 ⟨to_string⟩
+
+theorem bits_to_nat_of_to_bool (n : nat)
+: bitvec.bits_to_nat [to_bool (n % 2 = 1)] = n % 2
+:=
+   or.elim (nat.mod_2_or n)
+     (assume h : n % 2 = 0, begin rw h, refl end)
+     (assume h : n % 2 = 1, begin rw h, refl end)
+
+end bitvec
+
+section list
+
+open list
+open subtype
+
+theorem bitvec.bits_to_nat_over_append (xs : list bool) (y : bool)
+:  bitvec.bits_to_nat (xs ++ [y]) = bitvec.bits_to_nat xs * 2 + bitvec.bits_to_nat [y]  :=
+      begin
+        simp, unfold bitvec.bits_to_nat,
+        simp [foldl_to_cons],
+        unfold bitvec.add_lsb,
+        simp [nat.two_mul],
+      end
+
+end list
+
+namespace bitvec
+
+lemma div_mul_sub_one_cancel {n p k : ℕ} (Hp : 1 ≤ p)
+  (H : n ≤ p * p^k - 1)
+:  n / p ≤ p^k - 1 :=
+begin
+  assert H' : n / p ≤ (p*p^k - 1) / p,
+  { apply nat.div_le_div H _ },
+  rw nat.div_pred_to_pred_div (p^k) Hp at H',
+  apply H'
+end
+
+theorem bits_to_nat_list_of_nat
+: ∀ {k n : ℕ}, n ≤ 2 ^ k - 1 → bitvec.bits_to_nat (bitvec.list_of_nat k n) = n
+ | zero n :=
+        begin
+          intro Hn_le,
+          assert Hn_eq : n = 0,
+          { apply nat.le_zero_of_eq_zero Hn_le },
+          subst n, refl
+        end
+ | (nat.succ k) n :=
+        begin
+          intro H,
+          assert H' : n / 2 ≤ 2^k - 1,
+          { apply div_mul_sub_one_cancel (nat.le_succ _) H },
+          unfold bitvec.list_of_nat,
+          simp [ bitvec.bits_to_nat_over_append
+               , bits_to_nat_list_of_nat H'
+               , bits_to_nat_of_to_bool
+               , nat.mod_add_div n 2 ],
+        end
+
+theorem to_nat_of_nat {k n : ℕ} (h : n ≤ 2 ^ k - 1) :
+   bitvec.to_nat (bitvec.of_nat k n) = n
+:= by simp [to_nat_eq_bits_to_nat,bits_to_nat_list_of_nat h]
+
 end bitvec
 
 instance {n} {x y : bitvec n} : decidable (bitvec.ult x y) := bool.decidable_eq _ _
